proof/schnorr_protocol/W64_Zp_SchnorrIndistinguishability.ec
@@ -5,7 +5,7 @@ require import Array32 Array64 Array128.
 
 require import W64_SchnorrProtocol.
 require import Zp_SchnorrProtocol.
-
+require import AuxLemmas.
 
 require import Ring_ops_spec.
 import Zp DZmodP.
@@ -16,8 +16,7 @@ require import W64_SchnorrExtract.
 require import Ring_ops_proof.
 
 
-
-(* TODO: to check the constants to be right  *)
+(* TODO: proof constants to be correct  *)
 (* lemma bn_set_gg_value :  *)
 (*   phoare[ M.bn_set_gg : true ==> valR res =  1 ] = 1%r. *)
 (* proc. wp. skip. progress. simplify. *)
@@ -39,7 +38,6 @@ require import Ring_ops_proof.
 (* admit. *)
 (* rewrite /bn_seq. simplify. *)
 
-
 axiom bn_set_gg_prop : 
   phoare[ M.bn_set_gg : true ==> valR res = Sub.val g  ] = 1%r.
 
@@ -49,7 +47,7 @@ axiom bn_set_bf_prop :
   phoare[ M.bn_set_bf : true ==> W64x2N.valR res = Ri  ] = 1%r.
 
 axiom bn_set_eo_prop : 
-  phoare[ M.bn_set_eo : true ==> valR res = p-1  ] = 1%r.
+  phoare[ M.bn_set_eo : true ==> valR res = q  ] = 1%r.
 axiom bn_set_eb_prop : 
   phoare[ M.bn_set_eb : true ==> W64x2N.valR res = Rip  ] = 1%r.
 
@@ -62,20 +60,19 @@ lemma inzpKK: forall (z : int), val (inzmod z) = z %% p. smt(@Zp). qed.
   
 module ASpecFp_Schnorr = {
  proc commit(h : zmod, w : R) : zmod * int = {
-   var r, q : int;
+   var r;
    var a : zmod;    
-   r <@ ASpecFp.rsample(p-1);
+   r <@ ASpecFp.rsample(q);
    a <@ ASpecFp.expm(g,r);
    return (a,  r);
   } 
 
   proc challenge() : int = {
    var r;
-   r <@ ASpecFp.rsample(p-1);
+   r <@ ASpecFp.rsample(q);
    return r;
   }
 }.
-
 
 
 require import UniformSampling_Concrete.
@@ -95,12 +92,26 @@ call{1} bn_set_bf_prop.
 call{1} bn_set_gg_prop.
 call{1} bn_set_go_prop.
 call{1} bn_set_eo_prop.
-skip. move => &1 _ H r q r2 vr rr iz rp vri.
-split. smt.
+skip. move => &1 _ H r qe r2 vr rr iz rp vri.
+split. rewrite qe. simplify. smt(q_prime).
 move => h1. move => rL rR. move => rzrlrr. 
 split. 
 split.  smt. split. smt. split.  smt. split.  smt. rewrite /R. rewrite - vri. smt(@W64x2N @R2).
 move => qo. move => rl rrr ai. smt.
+qed.
+
+
+lemma exps (x : zmod) : forall n, 0 <= n => (x ^ n)%Ring_ops_spec = (x ^^ n). 
+apply intind. progress.
+smt(@Zp @Ring).
+progress.
+have ->: (x ^ (i + 1))%Ring_ops_spec = x * (x^ i)%Ring_ops_spec. 
+ rewrite /(^).
+ have ->: asint x ^ (i + 1) = (asint x) * (asint x ^ i). smt.
+ admit.
+have ->: (x ^^ (i + 1)) = x * (x^^i). smt.
+rewrite H0.
+auto.
 qed.
 
 
@@ -112,10 +123,9 @@ inline *. wp.  simplify. sp.
 rnd.
 skip. progress.  smt(@Distr).  
 rewrite - zp_eq.
-rewrite exps.
-rewrite /(^).
-rewrite inzpKK. congr. congr.
-rewrite /asint. auto.
+rewrite exps. smt(@DInterval).
+rewrite /(^^) /(^).
+auto.
 qed.
 
 lemma commitment_eq : 
@@ -130,86 +140,6 @@ transitivity ASpecFp_Schnorr.commit
     /\ res{1}.`2 = (valR res{2}.`2)). auto. auto.
 apply commit_same.
 symmetry. apply commit_same1.
-qed.
-
-require import ModularMultiplication_Concrete.
-require import BarrettReduction_Concrete.
-
-lemma verify_eq : 
-  equiv [ SchnorrVerifier.verify ~ JVerifier.verify :
-       Sub.val(s{1}) = valR statement{2} %% p
-       /\ Sub.val(z{1}) = valR commitment_0{2} %% p
-       /\ c{1} %% (p-1) = (valR (challenge_0{2})) %% (p-1)
-       /\ t{1} %% (p-1) = (valR response_0{2})  %% (p-1)
-       ==> (res{1} = (res{2} = W64.one)) /\ (res{2} = W64.zero \/ res{2} = W64.one) ].
-proc. sp. simplify.
-ecall {2} (bn_eq_correct v1{2} v2{2}). simplify. 
-ecall {2} (bn_expm_correct group_barrett{2} group_order{2} group_generator{2} response_0{2}). simplify. 
-ecall {2} (bn_mulm_correct commitment_0{2} tmp{2} group_order{2}). simplify.
-ecall {2} (bn_expm_correct group_barrett{2} group_order{2} statement{2} challenge_0{2}). simplify. 
-ecall {2} (bnreduce_small_spec_ph response_0{2} exp_order{2}). simplify.
-ecall {2} (bnreduce_small_spec_ph challenge_0{2} exp_order{2}). simplify.
-ecall {2} (bnreduce_small_spec_ph commitment_0{2} group_order{2}). simplify.
-ecall {2} (bnreduce_small_spec_ph statement{2} group_order{2}). simplify.
-call{2} bn_set_gg_prop.
-call{2} bn_set_bf_prop.
-call{2} bn_set_go_prop.
-call{2} bn_set_eb_prop.
-call{2} bn_set_eo_prop.
-simplify.
-skip. progress.
-rewrite ri_un. rewrite H6. rewrite Ri_def. rewrite /ri. smt().
-rewrite H5. smt(P_pos).
-smt(@W64xN).
-smt(@W64xN).
-rewrite H5. 
-smt.                            (* use p_val_prop1 *)
-smt(P_pos).
-smt(@W64xN).
-smt(@W64xN).
-rewrite H5. 
-smt.
-rewrite ri_un. rewrite H4. rewrite Rip_def. rewrite /ri. rewrite H3.
-smt(). 
-smt(P_pos).
-smt.
-smt(@W64xN).
-smt.
-smt(P_pos).
-smt.
-smt(@W64xN).
-smt.
-smt().
-rewrite /R. smt.
-smt(@W64xN).
-smt().
-smt(@W64xN).
-smt().
-smt(@Zp).
-rewrite H52. rewrite - H48. rewrite H51.
-rewrite H39.
-rewrite H3. rewrite - H2.
-rewrite H7.
-rewrite H23.
-rewrite H42.
-rewrite H15.
-rewrite H5.
-rewrite - H.
-rewrite - H0.
-rewrite H31.
-rewrite H3.
-rewrite - H1.
-rewrite - (zp_eq (z{1} * s{1} ^^ c{1}) (Ring_ops_spec.g ^^ t{1})).
-rewrite (exps Ring_ops_spec.g t{1}).
-rewrite (zp_mul).
-congr.
-congr.
-congr.
-congr.
-rewrite /P.
-rewrite - exps. smt(exp_pow). 
-rewrite - exps.
-rewrite /P. rewrite - exps. smt(exp_pow). 
 qed.
      
 
@@ -238,14 +168,21 @@ smt.
 qed.
 
 
+require import ModularMultiplication_Concrete.
+require import BarrettReduction_Concrete.
 
+axiom q_less_p      : q < p.
+axiom q_val_prop1 x : W64xN.valR x < q * q. 
+axiom p_val_prop2   : 2*p < W64xN.modulusR. 
+
+lemma p_val_prop1 x : W64xN.valR x < p * p.  by smt(q_less_p q_val_prop1 q_prime prime_p). qed.
 
 lemma response_eq : 
   equiv [ SchnorrProver.response ~ JProver.response :
-    w{1} %% (p-1)       = (valR (witness0{2}) )      %% (p-1)
-    /\ r{1} %% (p-1)    = (valR secret_power{2})     %% (p-1)
-    /\ c{1} %% (p-1)    = (valR challenge_0{2})      %% (p-1)
-    ==> res{1} %% (p-1)  = (valR res{2}) ].
+        w{1}   %% q  = (valR (witness0{2}) )  %% q
+    /\  r{1}   %% q  = (valR secret_power{2}) %% q
+    /\  c{1}   %% q  = (valR challenge_0{2})  %% q
+    ==> res{1} %% q  = (valR res{2}) ].
 proc. sp. simplify.
 ecall {2} (bn_addm_correct secret_power{2} product{2} exp_order{2}). simplify. 
 ecall {2} (bn_mulm_correct challenge_0{2} witness0{2} exp_order{2}). simplify.
@@ -260,13 +197,13 @@ progress. rewrite H3. rewrite Rip_def. rewrite ri_un. rewrite /ri. rewrite H2. s
 smt. 
 smt(@W64xN).
 smt(@W64xN).
-rewrite H2.   smt (p_val_prop1).
+rewrite H2.   smt (q_val_prop1).
 smt.
 smt.
 smt(@W64xN).
 smt.
 smt(@W64xN).
-rewrite H2. smt (p_val_prop1).
+rewrite H2. smt (q_val_prop1).
 smt(@W64xN).
 rewrite H2. smt.
 smt(@W64xN).
@@ -276,16 +213,97 @@ rewrite H2. smt.
 smt(@W64xN).
 rewrite H2. smt.
 smt(@W64xN).
-rewrite H2. smt (p_val_prop2).
+rewrite H2. smt (p_val_prop2 q_less_p).
 rewrite - H40.
 rewrite - H33.
 rewrite H2. 
-have -> : (r{1} + c{1} * w{1}) %% (p - 1)
-  = (r{1} %% (p - 1) + (c{1} * w{1}) %% (p - 1) ) %% (p - 1).
+have -> : (r{1} + c{1} * w{1}) %% q
+  = (r{1} %% q + (c{1} * w{1}) %% q ) %% q.
 smt (modzDmr modzDml).
 rewrite  H19 H2. rewrite - H0.
 rewrite  H11 H2. rewrite - H1.
 rewrite  H27 H2. rewrite - H.
 rewrite modzMml.
 rewrite modzMmr. done.
+qed.
+
+
+lemma verify_eq : 
+  equiv [ SchnorrVerifier.verify ~ JVerifier.verify :
+       Sub.val(s{1}) = valR statement{2} %% p
+       /\ Sub.val(z{1}) = valR commitment_0{2} %% p
+       /\ c{1} %% q = (valR (challenge_0{2})) %% q
+       /\ t{1} %% q = (valR response_0{2})  %% q
+       ==> (res{1} = (res{2} = W64.one)) /\ (res{2} = W64.zero \/ res{2} = W64.one) ].
+proc. sp. simplify.
+ecall {2} (bn_eq_correct v1{2} v2{2}). simplify. 
+ecall {2} (bn_expm_correct group_barrett{2} group_order{2} group_generator{2} response_0{2}). simplify. 
+ecall {2} (bn_mulm_correct commitment_0{2} tmp{2} group_order{2}). simplify.
+ecall {2} (bn_expm_correct group_barrett{2} group_order{2} statement{2} challenge_0{2}). simplify. 
+ecall {2} (bnreduce_small_spec_ph response_0{2} exp_order{2}). simplify.
+ecall {2} (bnreduce_small_spec_ph challenge_0{2} exp_order{2}). simplify.
+ecall {2} (bnreduce_small_spec_ph commitment_0{2} group_order{2}). simplify.
+ecall {2} (bnreduce_small_spec_ph statement{2} group_order{2}). simplify.
+call{2} bn_set_gg_prop.
+call{2} bn_set_bf_prop.
+call{2} bn_set_go_prop.
+call{2} bn_set_eb_prop.
+call{2} bn_set_eo_prop.
+simplify.
+skip. progress.
+rewrite ri_un. rewrite H6. rewrite Ri_def. rewrite /ri. smt().
+rewrite H5. smt(P_pos).
+smt(@W64xN).
+smt(@W64xN).
+rewrite H5. 
+have  : valR statement{2} < q * q.
+smt(q_val_prop1).
+have : q * q < p * p. smt(q_less_p q_prime prime_p @StdOrder).
+smt(p_val_prop1).
+smt(P_pos).
+smt(@W64xN).
+smt(@W64xN).
+rewrite H5. 
+smt.
+rewrite ri_un. rewrite H4. rewrite Rip_def. rewrite /ri. rewrite H3.
+smt(). 
+smt(q_prime).
+smt.
+smt(@W64xN).
+smt.
+smt(q_prime).
+smt.
+smt(@W64xN).
+smt.
+smt().
+rewrite /R. smt.
+smt(@W64xN).
+smt().
+smt(@W64xN).
+smt().
+smt(@Zp).
+rewrite H52. rewrite - H48. rewrite H51.
+rewrite H39.
+rewrite H3. rewrite - H2.
+rewrite H7.
+rewrite H23.
+rewrite H42.
+rewrite H15.
+rewrite H5.
+rewrite - H.
+rewrite - H0.
+rewrite H31.
+rewrite H3.
+rewrite - H1.
+rewrite - (zp_eq (z{1} * s{1} ^^ c{1}) (Zp_SchnorrProtocol.g ^^ t{1})).
+rewrite (exps Ring_ops_spec.g t{1}).
+rewrite (zp_mul).
+congr.
+congr.
+congr.
+congr.
+rewrite /P.
+rewrite - exps. smt(exp_pow). 
+rewrite - exps.
+rewrite /P. rewrite - exps. smt(exp_pow). 
 qed.
